---
aliases:
note-type: permanent
date-created: 2024-01-25
long-form-date-created: Thursday, January 25, 2024
week-created: Week 04.4
time-created: 01:23 PM
---

# 1.1 Systems of Linear Equations

Related :

## Example 01

> [!example]
>
> Consider the following system
>
> $$
> \begin{align*}
> x+2y=1 \\
> 3x+4y=-1
> \end{align*}
> $$

### (a) Is $\left(-3,1\right)$ a solution to the system?

❌ $\left(-3,1\right)$ is NOT a solution because it is not a solution to equation #2: $3x+4y=-1$

$\left(-3,1\right)$ is not a solution to $3x+4y=-1$

$$
\begin{align*}
3x+4y&=-1 \\
3\left(3\right)+4\left(1\right)&=-1 \\
9+4&=-1 \\
13&\overset{?}{=}1 \\13&\ne 1
\end{align*}
$$

#### What about $\left(-3,2\right)$?

✅ $\left(-3,2\right)$ is a solution to the system

$\left(-3,2\right)$ is a solution to $\large x+2y=1$

$$
\begin{align*}
x+2y&=1\\
\left(-3\right)+2\left(2\right)&=1\\
\left(-3\right)+4&=1\\
1&\overset{?}{=}1\\
1&=1 \checkmark\\
\end{align*}
$$

$\left(-3,2\right)$ is a solution to $\large 3x+4y=-1$

$$
\begin{align*}
3x+4y&=-1\\
3\left(-3\right)+4\left(2\right)&=-1\\
-9+8&=-1\\
-1&\overset{?}{=}-1\\
-1&=-1 \checkmark
\end{align*}
$$

### (b) Find <ins>all</ins> solutions to the system

**Use elimination**:

> [!info] Symbol Tilde: $\large \sim$
>
> The tilde is read as "equivalent": same solution set
>
> > [!example]
> >
> > $\huge \underset{-3r_1+r_2\rightarrow r_2}\sim$
>
> "r" means `row`, so $r_1$ is `row 1`

$$
\begin{align*}
x + 2y &= 1 \\ 3x + 4y &= -1
\end{align*}
\quad\LARGE\underset{-3r_1 + r_2 \rightarrow r_2}\sim
$$

> [!info] Scratch Work
>
> $$
> \begin{align*}
> &-3r_1&3x - 6y &= -3 \\
> &+r_2&3x + 4y &= -1 \\
> \hline
> &&0 - 2y &= -4 \\
> \end{align*}
> $$

$$
\begin{align*} x + 2y =& 1 \\ 2y =& -4 \end{align*}
\quad \LARGE\underset{-\frac{1}{2}r_2 \rightarrow r_2}\sim
$$

> [!attention] Solve This
>
> $$\begin{align*} x + 2y &= 1 \\ y &= 2 \end{align*}$$
>
> $\text{plug-and-chug using:}\:y=2 \quad \checkmark$
>
> $$\begin{align*} x+2\left(2\right)&=1 \\ \Rightarrow x&=-3 \end{align*}$$
>
> > [!done] Only one solution:
> >
> > $$
> > \begin{align*}
> > x &= -3 \\ y &= 2
> > \end{align*} \quad OR \quad \left(-3,2\right)
> > $$

### (c) Interpret the system geometrically

- Solutions to $x+2y=1$ are the points on the line it describes
- Similarly for $3x+4=-1$
- Solution(s) are the points on that line

Put into the standard from we get the following

$\begin{align*} x+2y&=1\\\Rightarrow \:y&=-\frac{1}{2}x+\frac{1}{2}\end{align*}$

$\begin{align*} 3x+4y&=1 \\ \Rightarrow y&=-\frac{1}{2}x+\frac{1}{2}\end{align*}$

When graphed we get the following

![Graph of the standard forms](../../attachments/Pasted%20image%2020240125160304.png)

When manipulating linear systems, we do not want to change the solution sets.

What are the allowable operations?

> [!note] Elementary Row Operations
>
> 1. **Replacement**: Replace a row by itself plus any multiple of another row $\large r_i+cr_j\rightarrow r_i$
> 2. **Interchange**: Swap any two rows $\large r_i \longleftrightarrow r_j$
> 3. **Scaling**: Multiply any row by a non-zero number $\large cr_i\rightarrow r_i$

If one system can be transformed into another by a series of row operations then we say:
the systems are **row equivalent**.

> [!info] Theorem
>
> If two systems are row equivalent, then they have the same solution sets

## Example Matrix Notation (by example)

Convert the system to augmented matrix form and then solve.

> [!example]
>
> $$
> \LARGE
> \begin{align*}
> x_1-3x_2=5 \\
> -x_1+x_2+5x_3=2 \\
> x_2+x_3=0
> \end{align*}
> $$

**Step 1)** Rewrite to align

$$
\large
\begin{alignedat}{3}
x_1&{}-{}&3x_2&&&=5 \\
-x_1&{}+{}&x_2&{}+{}&5x_3&=2 \\
&&x_2&{}+{}&x_3&=0
\end{alignedat}
$$

**Step 2)** Write in matrix form

$\LARGE{\begin{array}{ccc|c} & \begin{matrix}&x_1&x_2&x_3&&\quad\end{matrix} \\ & \left[\begin{array}{ccc|c} 1&-3&0&5\\-1&1&5&2\\0&1&1&0\end{array}\right]\\ \end{array}}$

**Step 3)** $\large r_1 + r_2 \rightarrow r_2$ - take `row 1` and add `row 2`; then, take the sum to replace `row 2`

> **Replacement**: Replace a row by itself plus any multiple of another row

$\LARGE{\left[\begin{array}{ccc|c} \enclose{circle}[mathcolor="blue"]{1} & -3 & 0 & 5 \\ -1 & 1 & 5 & 2 \\ 0 & 1 & 1 & 0 \\ \end{array} \right]{\underset{r_1 + r_2 \rightarrow r_2}\sim}\left[\begin{array}{ccc|c}\enclose{circle}[mathcolor="green"]{1} & -3 & 0 & 5 \\ 0 & \enclose{circle}[mathcolor="green"]{-2} & 5 & 7 \\ 0 & 1 & 1 & 0 \\ \end{array} \right]}$

**Step 4) $\large r_2 \longleftrightarrow r_3$** - swap `row 2` with `row 3`

> **Interchange**: Swap any two rows

$\LARGE{\left[\begin{array}{ccc|c}\enclose{circle}[mathcolor="green"]{1} & -3 & 0 & 5 \\ 0 & \enclose{circle}[mathcolor="green"]{-2} & 5 & 7 \\ 0 & 1 & 1 & 0 \\ \end{array} \right]\underset{r_2 \longleftrightarrow r_3}\sim} \left[\begin{array}{ccc|c}\enclose{circle}[mathcolor="green"]{1} & -3 & 0 & 5 \\ 0 & \enclose{circle}[mathcolor="green"]{1} & 1 & 0 \\ 0 & -2 & 5 & 7 \\ \end{array} \right]$

**Step 5) $\large 2r_2 + r_3 \rightarrow r_3$** - double `row 2` and add `row 3`; then, take the result to replace row 3

> **Replacement**: Replace a row by itself plus any multiple of another row

$\LARGE{\left[\begin{array}{ccc|c}\enclose{circle}[mathcolor="green"]{1} & -3 & 0 & 5 \\ 0 & \enclose{circle}[mathcolor="green"]{1} & 1 & 0 \\ 0 & -2 & 5 & 7 \\ \end{array} \right]{\underset{2r_2 + r_3 \rightarrow r_3}\sim} \left[\begin{array}{ccc|c}\enclose{circle}[mathcolor="green"]{1} & -3 & 0 & 5 \\ 0 & \enclose{circle}[mathcolor="green"]{1} & 1 & 0 \\ 0 & 0 & 7 & 7 \\ \end{array} \right]}$

**Step 6)** $\large \frac{1}{7}r_3\:\rightarrow\:r_3$ - scale down `row 3` by $\frac{1}{7}$ (i.e. divide `row 3` by 7)

> **Scaling**: Multiply any row by a non-zero number

${\LARGE{\left[\begin{array}{ccc|c}\enclose{circle}[mathcolor="green"]{1} & -3 & 0 & 5 \\ 0 & \enclose{circle}[mathcolor="green"]{1} & 1 & 0 \\ 0 & 0 & 7 & 7 \\ \end{array} \right]\underset{\frac{1}{7}r_3\:\rightarrow\:r_3}\sim} \left[\begin{array}{ccc|c}\enclose{circle}[mathcolor="green"]{1} & -3 & 0 & 5 \\ 0 & \enclose{circle}[mathcolor="green"]{1} & 1 & 0 \\ 0 & 0 & \enclose{circle}[mathcolor="green"]{1} & 1 \\ \end{array} \right]}$

This is to say that the original system is equitant to

$Original\\\Huge{\begin{array}{ccc|c} & \begin{matrix}&x_1&x_2&x_3&&\quad\end{matrix} \\ & \left[\begin{array}{ccc|c} 1 & -3 & 0 & 5 \\ -1 & 1 & 5 & 2 \\ 0 & 1 & 1 & 0 \\ \end{array}\right]\\ \end{array} \underset{is\:equivalent\:to}{\sim} \begin{array}{ccc|c} & \begin{matrix}&x_1&x_2&x_3&&\quad\end{matrix} \\ & \left[\begin{array}{ccc|c} 1 & -3 & 0 & 5 \\ 0 & 1 & 1 & 0 \\ 0 & 0 & 1 & 1 \\ \end{array}\right]\\ \end{array}}\\ Modified$

Modified

$\begin{alignedat}{3} Equation\:\enclose{circle}[mathcolor="black"]{1} \quad x_1&{}-{}&3x_2&&&=5& \\ Equation\:\enclose{circle}[mathcolor="black"]{2} \qquad &&x_2&{}+{}&x_3&=0& \\ Equation\:\enclose{circle}[mathcolor="black"]{3} \qquad &&&&x_3&=1& \end{alignedat}$

**Step 7)** Finish solving

$\begin{alignedat}{3} Equation\:\enclose{circle}[mathcolor="black"]{1}\:&x_1-3\left(-1\right)=5\\&\Rightarrow x_1=2 \\  \\Equation\:\enclose{circle}[mathcolor="black"]{2}\:&2x+1=0\\ &\Rightarrow x_2=-1\\  \\Equation\:\enclose{circle}[mathcolor="black"]{3}\:&x_3=1 \end{alignedat}$

> [!done]
>
> $\begin{align}  x_1=\:&2 \\ x_2=\:&-1 \\ x_3=\:&1 \\ \end{align} \quad OR \quad {\large \left(2,-1,1\right)}$

## Example: Determine if the follow is consistent

`consistent`: There is at least one solution

Using the elimination method

> [!example]
>
> $$
> \LARGE
> \begin{align*}
> x+y&=1 \\
> x+2y&=2 \\
> -x+3y&=7
> \end{align*}
> $$

**Step 1)** Write in matrix form

> Reduce: make zeros

$$
\LARGE
\begin{array}{ccc|c}
&\begin{matrix}\qquad
&x&y&=&&
\quad\end{matrix}\\
&\left[
\begin{array}{cc|c}
    \enclose{circle}[mathcolor="blue"]{1}&1&1\\
    1&2&2\\
    -1&3&7
\end{array}
\right]
\\\end{array}
$$

**Step 2)** $\Large -r_1\:+\:r_2\:\rightarrow\:r_2$ make `row 1` negative of the same values and take the sum
of `row 1` and `row 2`; after, $\Large r_1\:+\:r_3\:\rightarrow\:r_3$ add `row 1` and `row 3`, and use the sum to
replace `row 3`

> **Replacement**: Replace a row by itself plus any multiple of another row

$$
\Huge
\left[
\begin{array}{cc|c}
    \enclose{circle}[mathcolor="blue"]{1}&1&1\\
    1&2&2\\
    -1&3&7\\
\end{array}
\right]
\underset{\begin{align*}
    -r_1\:+\:r_2\:\rightarrow\:r_2\\
    r_1\:+\:r_3\:\rightarrow\:r_3
\end{align*}}\sim

\left[
\begin{array}{cc|c}
    \enclose{circle}[mathcolor="blue"]{1}&1&1\\
    0&\enclose{circle}[mathcolor="blue"]{1}&1\\
    0&4&8\\
\end{array}
\right]
$$

**Step 3)** $\Large -4r_2\:+\:r_3\:\rightarrow\:r_3$ multiply `row 2` by $-4$ then add `row 2` with `row 3`;
after, take the sum and replace it with `row 3`

> **Replacement**: Replace a row by itself plus any multiple of another row

$$
\Huge
\left[
\begin{array}{cc|c}
    \enclose{circle}[mathcolor="blue"]{1}&1&1\\
    0&\enclose{circle}[mathcolor="blue"]{1}&1\\
    0&4&8\\
\end{array}
\right]
\underset{-4r_2\:+\:r_3\:\rightarrow\:r_3}\sim
\left[
\begin{array}{cc|c}
    \enclose{circle}[mathcolor="blue"]{1}&1&1\\
    0&\enclose{circle}[mathcolor="blue"]{1}&1\\
    \fbox{0}&\fbox{4}&\fbox{8}\\
\end{array}
\right]
$$

**All together**:

$$
\large{
\left[
\begin{array}{cc|c}
    \enclose{circle}[mathcolor="blue"]{1}&1&1\\
    1&2&2\\
    -1&3&7\\
\end{array}
\right]
\underset{\begin{align*}
    -r_1\:+\:r_2\:\rightarrow\:r_2\\
    r_1\:+\:r_3\:\rightarrow\:r_3
\end{align*}}\sim

\left[
\begin{array}{cc|c}
    \enclose{circle}[mathcolor="blue"]{1}&1&1\\
    0&\enclose{circle}[mathcolor="blue"]{1}&1\\
    0&4&8\\
\end{array}
\right]
\underset{-4r_2\:+\:r_3\:\rightarrow\:r_3}\sim

\left[
\begin{array}{cc|c}
    \enclose{circle}[mathcolor="blue"]{1}&1&1\\
    0&\enclose{circle}[mathcolor="blue"]{1}&1\\
    \fbox{0}&\fbox{4}&\fbox{8}\\
\end{array}
\right]
}
$$

> [!done]
>
> $$
> \LARGE
> \begin{align*}
> x+y&=1 \\
> y&=1 \\
> 0&=4 \\
> \text{No Solutions}&\therefore\:\fbox{Inconsistent}
> \end{align*}
> $$

$$
\left.
\begin{align*}
        x+y=1 \\
        y=1 \\
        0=4 \\
\end{align*}
\right\}\:\text{Geometrically 3 lines in $\mathbb{R}^2$}
$$

## Example: Find all solutions

> [!example]
>
> $$
> \LARGE
> \begin{align*}
> 2x-y+3z&=4 \\
> 2x+3y-5z&=0 \\
> \end{align*}
> $$

**Step 1)** Write in matrix form

$$
\Huge
\left[
\begin{array}{ccc|c}
    2&-1&3&4\\
    2&3&-5&0\\
\end{array}
\right]
$$

**Step 2)** $\Large{-r_1\:+\:r_2\:\rightarrow\:r_2}$ multiply `row 1` with $-1$, add `row 2`, and replace the sum with `row 2`

> **Replacement**: Replace a row by itself plus any multiple of another row

$$
\Huge
\left[
\begin{array}{ccc|c}
    \enclose{circle}[mathcolor="blue"]{2}&-1&3&4\\
    2&3&-5&0\\
\end{array}
\right]
\underset{-r_1\:+\:r_2\:\rightarrow\:r_2}\sim
\left[
\begin{array}{ccc|c}
    \enclose{circle}[mathcolor="blue"]{2}&-1&3&4\\
    0&4&-8&-4\\
\end{array}
\right]
$$

**Step 3)** $\Large{\frac{1}{4}r_2\:\rightarrow \:r_2}$ replace `row 2` with a $\frac{1}{4}$ scale-down version of `row 2`

> **Scaling**: Multiply any row by a non-zero number

$$
\Huge
\left[
\begin{array}{ccc|c}
    \enclose{circle}[mathcolor="blue"]{2}&-1&3&4\\
    0&4&-8&-4\\
\end{array}
\right]
\underset{\frac{1}{4}r_2\:\rightarrow \:r_2}\sim
\left[
\begin{array}{ccc|c}
    \enclose{circle}[mathcolor="blue"]{2}&-1&3&4\\
    0&\enclose{circle}[mathcolor="blue"]{1}&-2&-1\\
\end{array}
\right]
$$

**So, all together - steps 2 & 3**:

$$
\
\left[
\begin{array}{ccc|c}
    \enclose{circle}[mathcolor="blue"]{2}&-1&3&4\\
    2&3&-5&0\\
\end{array}
\right]
\underset{-r_1\:+\:r_2\:\rightarrow\:r_2}\sim
\left[
\begin{array}{ccc|c}
    \enclose{circle}[mathcolor="blue"]{2}&-1&3&4\\
    0&4&-8&-4\\
\end{array}
\right]
\underset{\frac{1}{4}r_2\:\rightarrow \:r_2}\sim
\left[
\begin{array}{ccc|c}
    \enclose{circle}[mathcolor="blue"]{2}&-1&3&4\\
    0&\enclose{circle}[mathcolor="blue"]{1}&-2&-1\\
\end{array}
\right]
$$

$$
\LARGE
\left.
\begin{align*}
2x-y+3z=4\\
y-2z=-1\\
\end{align*}
\right\}
\Rightarrow

\left.
\begin{alignedat}{3}
2x=4+\fbox{y}-3z\\
\fbox{y=-1+2z}
\end{alignedat}
\right\}
\Rightarrow

\begin{alignedat}{3}
x&=\frac{3}{2}-\frac{1}{2}z\\
y&=-1+2z\\
&\text{z is free}
\end{alignedat}
$$

> [!done]
>
> $$
> \LARGE
> \begin{align*}
> x&=\frac{3}{2}-\frac{1}{2}z\\
> y&=-1+2z\\
> &\text{z is free}
> \end{align*}
> $$

**Example solution**:

$\LARGE\left(\frac{3}{2}-\frac{7}{2},\:-1+14,\:7\right),\:\left(\frac{3}{2}-\frac{\pi }{2},-1+2\pi ,\pi \right),\dots$

## Final Remark

A linear system can have $0,\:1,\:\infty$-many solutions; that is to say, having exactly 2
solutions is not possible.
